silveroak-opentitan/aes/Spec/CommuteProperties.v
@@ -1,0 +1,72 @@
+(****************************************************************************)
+(* Copyright 2020 The Project Oak Authors                                   *)
+(*                                                                          *)
+(* Licensed under the Apache License, Version 2.0 (the "License")           *)
+(* you may not use this file except in compliance with the License.         *)
+(* You may obtain a copy of the License at                                  *)
+(*                                                                          *)
+(*     http://www.apache.org/licenses/LICENSE-2.0                           *)
+(*                                                                          *)
+(* Unless required by applicable law or agreed to in writing, software      *)
+(* distributed under the License is distributed on an "AS IS" BASIS,        *)
+(* WITHOUT WARRANTIES OR CONDITIONS OF ANY KIND, either express or implied. *)
+(* See the License for the specific language governing permissions and      *)
+(* limitations under the License.                                           *)
+(****************************************************************************)
+
+Require Import Coq.Init.Byte.
+Require Import Coq.Lists.List.
+
+Require Import AesSpec.ShiftRows.
+Require Import AesSpec.SubBytes.
+Require Import AesSpec.Sbox.
+
+Section Spec.
+  Section Properties.
+    Lemma sub_byte_shift_row_once_comm : forall row,
+      shift_row_once (map forward_sbox row) =
+      map forward_sbox (shift_row_once row).
+    Proof.
+      intros.
+      destruct row; [reflexivity|].
+      simpl.
+      rewrite map_app.
+      reflexivity.
+    Qed.
+
+    Lemma sub_byte_shift_row_comm : forall row shift,
+      shift_row (map forward_sbox row) shift =
+      map forward_sbox (shift_row row shift).
+    Proof.
+      intros.
+      generalize dependent row.
+      induction shift; [reflexivity|].
+      intros.
+      simpl.
+      rewrite <- IHshift.
+      rewrite sub_byte_shift_row_once_comm.
+      reflexivity.
+    Qed.
+
+    Lemma sub_bytes_shift_rows_start_comm : forall st n,
+      shift_rows_start (sub_bytes st) n =
+      sub_bytes (shift_rows_start st n).
+    Proof.
+      induction st; [reflexivity|].
+      intro n.
+      unfold shift_rows_start.
+      simpl.
+      rewrite sub_byte_shift_row_comm.
+      unfold shift_rows_start in IHst.
+      rewrite IHst.
+      reflexivity.
+    Qed.
+
+    Theorem sub_bytes_shift_rows_comm : forall st,
+      shift_rows (sub_bytes st) = sub_bytes (shift_rows st).
+    Proof.
+      intros.
+      apply (sub_bytes_shift_rows_start_comm st 0).
+    Qed.
+  End Properties.
+End Spec.
